completeness.thy
@@ -15,87 +15,50 @@ lemma completeness_1:
   assumes step_s: "S ~~ (i, a, False) \<leadsto>\<^sub>S S'"
     and wf: "state_wellFormed S"
   shows "\<exists>tr. (initialState (prog S) ~~ tr \<leadsto>* S') \<and> (i,a) \<in> set tr" 
-proof (cases a)
-next
-  case AEndAtomic
-  with step_s
-  have "S ~~ (i, a) \<leadsto> S'"
-    by (auto simp add: step_s.simps step.simps)
-  obtain tr where "initialState (prog S) ~~ tr \<leadsto>* S"
-    using local.wf state_wellFormed_def by blast
+proof (cases "\<exists>p. a = AInvoc p")
+  case True
+  from this obtain p where "a = AInvoc p" by blast
 
-  with `S ~~ (i, a) \<leadsto> S'`
-  have "initialState (prog S) ~~ tr@[(i,a)] \<leadsto>* S'"
-    using wf state_wellFormed_def steps_step by blast
+  from `a = AInvoc p` step_s
+  show "\<exists>tr. (initialState (prog S) ~~ tr \<leadsto>* S') \<and> (i, a) \<in> set tr"
+  proof (auto simp add: step_s.simps, fuzzy_goal_cases InvocStep)
+    case (InvocStep initState impl S_invoc)
 
-  thus ?thesis
-    by auto
-next
-  case (AReturn r)
-  with step_s
-  have "S ~~ (i, a) \<leadsto> S'"
-    by (auto simp add: step_s.simps step.simps)
-  obtain tr where "initialState (prog S) ~~ tr \<leadsto>* S"
-    using local.wf state_wellFormed_def by blast
+    have h1: "localState S_invoc i = None"
+      by (simp add: InvocStep.invocationOp_eq2 InvocStep.state_wellFormed wf_localState_needs_invocationOp)
 
-  with `S ~~ (i, a) \<leadsto> S'`
-  have "initialState (prog S) ~~ tr@[(i,a)] \<leadsto>* S'"
-    using wf state_wellFormed_def steps_step by blast
+    from h1 
+    have "S_invoc ~~ (i,a) \<leadsto> S'"
+      by (auto simp add: step.simps  InvocStep)
 
-  thus ?thesis
-    by auto
-next
-  case (AInvoc p)
-  show ?thesis
-  proof (rule ccontr)
-    assume "\<nexists>tr. (initialState (prog S) ~~ tr \<leadsto>* S') \<and> (i, a) \<in> set tr "
+    from `state_wellFormed S_invoc`
+    obtain tr1 where "initialState (prog S) ~~ tr1 \<leadsto>* S_invoc"
+      using state_wellFormed_def ` prog S_invoc = prog S` by metis
 
-    from AInvoc step_s
-    show False
-    proof (auto simp add: step_s.simps, fuzzy_goal_cases InvocStep)
-      case (InvocStep initState impl S_invoc)
-      
-      have h1: "localState S_invoc i = None"
-        by (simp add: InvocStep.invocationOp_eq2 InvocStep.state_wellFormed wf_localState_needs_invocationOp)
-
-      have "\<And>x. x \<in> uniqueIds p \<Longrightarrow> x \<in> knownIds S_invoc"
-        using InvocStep.less_eq by blast
-
-      from h1 
-      have "S_invoc ~~ (i,a) \<leadsto> S'"
-        by (auto simp add: step.simps  InvocStep)
-
-      from `state_wellFormed S_invoc`
-      obtain tr1 where "initialState (prog S) ~~ tr1 \<leadsto>* S_invoc"
-        using state_wellFormed_def ` prog S_invoc = prog S` by metis
-
-      with `S_invoc ~~ (i,a) \<leadsto> S'`
-      show ?case
-        using \<open>\<nexists>tr. (initialState (prog S) ~~ tr \<leadsto>* S') \<and> (i, a) \<in> set tr\<close> steps_step by force
-    qed
+    with `S_invoc ~~ (i,a) \<leadsto> S'`
+    show ?case
+      by (auto simp add: InvocStep.a_def InvocStep.S'_def steps_step intro!: exI[where x="tr1@[(i,a)]"])
   qed
-next
-  case (ALocal ok)
+next 
+  case False
+  text "Other cases are: endAtomic, local, return. 
+    For these we can exactly reproduce the step:"
 
-  from ALocal `S ~~ (i, a, False) \<leadsto>\<^sub>S S'`
-  have "ok = False"
+  from step_s False
+  have "S ~~ (i, a) \<leadsto> S'"
     by (auto simp add: step_s.simps)
+      (auto simp add: step.simps intro!: exI)
 
-  from ALocal `S ~~ (i, a, False) \<leadsto>\<^sub>S S'` 
-  have a: "S ~~ (i, a) \<leadsto> S'"
-    by (auto simp add: step_s.simps step.simps)
-
-  obtain tr where b: "initialState (prog S) ~~ tr \<leadsto>* S"
+  obtain tr where "initialState (prog S) ~~ tr \<leadsto>* S"
     using local.wf state_wellFormed_def by blast
 
   with `S ~~ (i, a) \<leadsto> S'`
-  have "initialState (prog S) ~~ tr@[(i, a)] \<leadsto>* S'"
-    using steps_step by blast
+  have "initialState (prog S) ~~ tr@[(i,a)] \<leadsto>* S'"
+    using wf state_wellFormed_def steps_step by blast
 
-
-  thus "?thesis"
+  thus ?thesis
     by auto
-qed (insert assms, auto simp add: step_s.simps)
+qed
 
 
 theorem completeness:
